\linespread{1.5}

\textbf{Solução}

Seja:

\begin{equation*}
    \begin{cases}
    u_x = pcos(px+t)-sin(x+qt)\\
    u_{xx} = -p^2sin(px+t) - cos(x+qt)\\
    u_t = cos(px+t) - qsin(x+qt)\\
    u_{tt} = -sin(px+t) -q^2cos(x+qt)
    \end{cases}
\end{equation*}

substituindo as expressões das segundas derivadas na equação de onda:
\begin{equation*}
    u_{tt} = -sin(px+t) -q^2cos(x+qt) = a^2(-p^2sin(px+t) - cos(x+qt)) = a^2u_xx
\end{equation*}
Para que a igualdade seja verdadeira temos que:
\begin{equation*}
    \begin{cases}
    (ap)^2 = 1\\
    q^2 = a^2
    \end{cases}
    \longrightarrow
    \begin{cases}
    p = \pm a^-1\\
    q = \pm a
    \end{cases}
\end{equation*}