\linespread{1.5}

\textbf{Solução}

Fazemos as derivadas em relação a $x$ e $y$:
\begin{equation*}
    u_x = 5ax^4 + 4bx^3y + 3cx^2y^2 + 2sxy^3 + ey^4
\end{equation*}
\begin{equation*}
    u_{xx} = 20ax^3 + 12bx^2y + 6cxy^2 + 2dy^3
\end{equation*}
\begin{equation*}
    u_y = bx^4 + 2cx^3y + 3dx^2y^2 + 4exy^3 + 5fy^4
\end{equation*}
\begin{equation*}
    u_{yy} = 2cx^3 + 6dx^2y + 12exy^2 + 20fy^3
\end{equation*}

Substituindo na equação de Laplace e divindo a mesma por 2:

\begin{equation*}
    10ax^3 + 6bx^2y + 3cxy^2 + dy^3 + cx^3 + 3dx^2y + 6exy^2 + 10fy^3 = 0
\end{equation*}

\begin{equation*}
    x^3(10a+c) + x^2y(6b+3d) + xy^2(3c+6e) + y^3(d+10f) = 0
\end{equation*}
\begin{equation*}
    \begin{cases}
    10a+c = 0\\
    6b+3d = 0\\
    3c+6e = 0\\
    d + 10f = 0
    \end{cases}
    \Rightarrow \begin{cases}
    \boxed{c = -10a}\\
    \boxed{d = -2b} \\
    c = -2e \rightarrow \boxed{e = 5a}\\
    d = -10f \rightarrow \boxed{f = \frac{b}{5}}
    \end{cases}
\end{equation*}

Assim:
\begin{equation*}
    u(x,y) = ax^5 + bx^4y -10ax^3y^2 - 2bx^2y^3 + 5axy^4 + \frac{b}{5}y^5
\end{equation*}
\begin{equation*}
    \boxed{u(x, y) = a(x^5 - 10x^3y^2 + 5xy^4) + b\left(x^4y - 2bx^2y^3 + \frac{1}{5}y^5\right)}
\end{equation*}