\linespread{1.5}
Determine a solução das seguintes equações diferenciais de primeira ordem:
\begin{itemize}
    \item[\textbf{a)}] $\frac{dy}{dx} - 3y\cos{x} = 0$;
    \item[\textbf{b)}] $\frac{dy}{dx} = \frac{xy^3}{\sqrt{1+x^2}}$;
    \item[\textbf{c)}] $\frac{dy}{dx} = e^{2x+y}$;
    \item[\textbf{d)}] $\frac{dy}{dx} = \frac{xy}{1+x}$;
    \item[\textbf{e)}] $x\sin^2{y}\frac{dy}{dx} = (x+1)^2$;
    \item[\textbf{f)}] $xy^4dx + (y^2+2)e^{-3x}dy = 0$;
    \item[\textbf{g)}] $\frac{dy}{dx} = \frac{x-e^{-x}}{y+e^y}$;
    \item[\textbf{h)}] $(1+y)x - (1+x)\frac{dy}{dx} = 0$;
    \item[\textbf{i)}] $\frac{dy}{dx} = 1 + x + y^2 + xy^2$;
    \item[\textbf{j)}] $\frac{dy}{dx} + ycos(x) = 0$;
    \item[\textbf{k)}] $\frac{dy}{dx} = \frac{1 + y^2}{1+x^2}$;
    \item[\textbf{l)}] $\frac{dy}{dx} = \frac{1+y^2}{(1+x^2)xy}$ ;
    \item[\textbf{m)}] $\frac{dy}{dx} = 3x -1$;
    \item[\textbf{n)}] $\frac{dy}{dx} = y^2-4$;
    \item[\textbf{o)}] $\frac{dy}{dx} = \frac{e^{-2y}}{x^2+4}$;
    \item[\textbf{p)}] $x\dot{y} = y + 2x^3sin^2\left(\frac{y}{x}\right)$;
    \item[\textbf{q)}] $x\dot{y} = y^2 + y$;
    \item[\textbf{r)}] $x\dot{y} = y + 3x^4cos^2\left(\frac{y}{x}\right)$;
    
\end{itemize}