\linespread{1.5}
Resolva as seguites equações diferenciais ordinárias de 2ª ordem:
\begin{itemize}
    \item[\textbf{a)}] $9y'' + 9y' - 4y=0$;
    \item[\textbf{b)}] $y''+y'-2y=2x$;
    \item[\textbf{c)}] $2y''+3y'+y=x² + 3sin(x)$;
    \item[\textbf{d)}] $y'' + 4y' = x^2 + 3e^x$;
    \item[\textbf{e)}] $y'' + 2y' = 3 + 4sin(2x)$;
    \item[\textbf{f)}] $y'' + 2y' + 5y = e^{-x}cos(2x)$;
    \item[\textbf{g)}] $y'' - y' - 2y = cosh(2x)$;
    \item[\textbf{h)}] $y'' + 4y = sec^2(2x)$;
    \item[\textbf{i)}] $y'' - 2y' - 8y = 4e^{2x} - 21e^{-3x}$;
    \item[\textbf{j)}] $y'' - 3y' + 2y = 4x^2$;
    \item[\textbf{k)}] $y'' - 6y' + 8y = 0$;
    \item[\textbf{l)}] $y'' - 2y' - 3y = 0$;
    \item[\textbf{m)}] $y'' - 9y = 0$;
    \item[\textbf{n)}] $\ddot{y} + y = sec(x)$, $0 < x < \frac{\pi}{2}$;
    \item[\textbf{o)}] $x^2y'' - 3xy' + 4y = x^4$, $x>0$;
    \item[\textbf{p)}] $y'' - y' + 5y = 3$;
    \item[\textbf{q)}] $y'' - 3y' - 4y = 3e^{2x}$;
    \item[\textbf{r)}] $y'' - 3y' - 4y = 2sin(x)$;
    \item[\textbf{s)}] $y'' - 3y' - 4y = -8e^xcos(2x)$;
    \item[\textbf{t)}] $y'' + 4y = 3cos(2x)$;
    \item[\textbf{u)}] $y'' - 4y' = x^2 + x$;
    \item[\textbf{v)}] $y'' + 3y' + 2y = 12x$;
    \item[\textbf{w)}] $y'' + 4y' + 4y = e^{-x}cos(x)$;
    \item[\textbf{x)}] $x^2\ddot{y} - 20y = 0$;
    \item[\textbf{y)}] $4x^2\ddot{y} - 5y = 0$;
    \item[\textbf{z)}] $y'' + 4y' + (\pi + 4)y = 0$;
\end{itemize}