\linespread{1.5}
Determine o original correspondente Ã s seguintes imagens utilizando as propriedades da transformada de Laplace:
\begin{itemize}
    \item[\textbf{a)}] {\Large $F(s) = \frac{3-s^2}{s^4}$}
    \item[\textbf{b)}] {\Large $F(s) = \frac{s+3}{(s-4)^2 + 4}$}
    \item[\textbf{c)}] {\Large $F(s) = \frac{s-2}{(s-3)(s-4)}$}
    \item[\textbf{d)}] {\Large $F(s) = \frac{e^{3s}-1}{se^{3s}}$}
    \item[\textbf{e)}] {\Large $F(s) = \frac{se^{-3s}}{(s-3)(s-4)}$}
    \item[\textbf{f)}] {\Large $F(s) = \frac{-6}{(s-3)^3}$}
    \item[\textbf{g)}] {\Large $F(s) = \frac{5s + 1}{s^2 -25}$}
    \item[\textbf{h)}] {\Large $F(s) = \frac{1}{(s+\sqrt{2})(s-\sqrt{3})}$}
    \item[\textbf{i)}] {\Large $F(s) = \frac{1}{(s+a)(s+b)}$}
    \item[\textbf{j)}] {\Large $F(s) = \frac{1}{s^2 - 4s + 5}$}
    \item[\textbf{k)}] {\Large $F(s) = \arctan{\frac{1}{s}}$}
\end{itemize}