\linespread{1.5}
\textbf{Solução}
iniciamos determinando $f(x)$ e $g(x)$
\begin{equation*}
    f(x) = a_0 + \sum_{n=1}^\infty a_n\cos{(nw_fx)} + b_n\sin{(nw_fx)}
\end{equation*}

\begin{equation*}
    g(x) = c_0 + \sum_{n=1}^\infty c_n\cos{(nw_gx)} + d_n\sin{(nw_gx)}
\end{equation*}

Agora multiplicamos $f(x)$ por $k$ e $g(x)$ por $m$

\begin{equation*}
    kf(x) = ka_0 + \sum_{n=1}^\infty ka_n\cos{(nw_fx)} + kb_n\sin{(nw_fx)}
\end{equation*}

\begin{equation*}
    mg(x) = mc_0 + \sum_{n=1}^\infty mc_n\cos{(nw_gx)} + md_n\sin{(nw_gx)}
\end{equation*}

Somamos então $kf(x)$ e $mg(x)$:

\begin{equation*}
    kf(x) + mg(x) = ka_0 + \sum_{n=1}^\infty ka_n\cos{(nw_fx)} + kb_n\sin{(nw_fx)} + mc_0 + \sum_{n=1}^\infty mc_n\cos{(nw_gx)} + md_n\sin{(nw_gx)}
\end{equation*}

Se o período f(x) for igual ao período de g(x), então $w_f = w_g = w$. Logo:

\begin{equation*}
    kf(x) + mg(x) = (ka_0 + mc_0) + \sum_{n=1}^\infty (ka_n + mc_n)\cos{(nwx)} + (kb_n + md_n)\sin{(nwx)}
\end{equation*}

ou seja, a função $kf(x) + mg(x)$ tem os seguintes coeficientes de Fourier:
\begin{equation*}
    \boxed{ka_0 + mc_0} \hspace{3cm}
    \boxed{ka_n + mc_n}
    \hspace{3cm}
    \boxed{kb_n + md_n}
\end{equation*}

c.q.d